updates

generic/Zeta.Generic.Blum.fst
@@ -1,12 +1,77 @@
 module Zeta.Generic.Blum
 
+module IF = Zeta.IdxFn
+
+let gen_seq (vspec n:_) = {
+  IF.seq_t = verifiable_log vspec n;
+  IF.length = length;
+  IF.prefix = prefix;
+}
+
+(* is this a blum add within epoch ep *)
+let is_blum_add_epoch (#vspec #n:_) (ep: epoch) (il: verifiable_log vspec n) (i: seq_index il)
+  = is_blum_add il i &&
+    (let be = blum_add_elem il i in
+     be.t.e = ep)
+
+let is_blum_add_epoch_ifn (#vspec #n:_) (ep: epoch)
+  : IF.idxfn_t (gen_seq vspec n) bool
+  = is_blum_add_epoch #vspec #n ep
+
+let is_blum_add_ifn (#vspec #n:_)
+  : IF.idxfn_t (gen_seq vspec n) bool
+  = is_blum_add #vspec #n
+
+let blum_add_elem_ifn (#vspec #n:_)
+  : IF.cond_idxfn_t (ms_hashfn_dom vspec.app) (is_blum_add_ifn #vspec #n)
+  = blum_add_elem #vspec #n
+
+let blum_add_elem_src (#vspec #n:_) (il: verifiable_log vspec n) (i: seq_index il{is_blum_add il i})
+  : elem_src (ms_hashfn_dom vspec.app) n
+  = let e = blum_add_elem il i in
+    let s = src il i in
+    {e ; s}
+
+let blum_add_elem_src_ifn (#vspec #n:_)
+  : IF.cond_idxfn_t (elem_src (ms_hashfn_dom vspec.app) n) (is_blum_add_ifn #vspec #n)
+  = blum_add_elem_src #vspec #n
+
 let add_il (#vspec #n:_) (ep: epoch) (il: verifiable_log vspec n)
   : interleaving (ms_hashfn_dom vspec.app) n
-  = admit()
+  = let fm = IF.to_fm (is_blum_add_epoch_ifn #vspec #n ep) (blum_add_elem_src_ifn #vspec #n) in
+    IF.filter_map fm il
+
+let is_blum_evict_epoch (#vspec #n:_) (ep: epoch) (il: verifiable_log vspec n) (i: seq_index il)
+  = is_blum_evict il i &&
+    (let be = blum_evict_elem il i in
+     be.t.e = ep)
+
+let is_blum_evict_epoch_ifn (#vspec #n:_) (ep: epoch)
+  : IF.idxfn_t (gen_seq vspec n) bool
+  = is_blum_evict_epoch #vspec #n ep
+
+let is_blum_evict_ifn (#vspec #n:_)
+  : IF.idxfn_t (gen_seq vspec n) bool
+  = is_blum_evict #vspec #n
+
+let blum_evict_elem_ifn (#vspec #n:_)
+  : IF.cond_idxfn_t (ms_hashfn_dom vspec.app) (is_blum_evict_ifn #vspec #n)
+  = blum_evict_elem #vspec #n
+
+let blum_evict_elem_src (#vspec #n:_) (il: verifiable_log vspec n) (i: seq_index il{is_blum_evict il i})
+  : elem_src (ms_hashfn_dom vspec.app) n
+  = let e = blum_evict_elem il i in
+    let s = src il i in
+    { e; s }
+
+let blum_evict_elem_src_ifn (#vspec #n:_)
+  : IF.cond_idxfn_t (elem_src (ms_hashfn_dom vspec.app) n) (is_blum_evict_ifn #vspec #n)
+  = blum_evict_elem_src #vspec #n
 
 let evict_il (#vspec #n:_) (ep: epoch) (il: verifiable_log vspec n)
   : interleaving (ms_hashfn_dom vspec.app) n
-  = admit()
+  = let fm = IF.to_fm (is_blum_evict_epoch_ifn #vspec #n ep) (blum_evict_elem_src_ifn #vspec #n) in
+    IF.filter_map fm il
 
 let lemma_add_evict_set_identical_glog (#vspec #n:_) (epmax: epoch) (il: verifiable_log vspec n)
   : Lemma (ensures (aems_equal_upto epmax il <==> G.aems_equal_upto epmax (to_glog il)))
@@ -16,7 +81,16 @@ let add_set_contains_each_add_elem (#vspec #n:_) (il: verifiable_log vspec n) (i
   : Lemma (ensures (let be = blum_add_elem il i in
                     let ep = be.t.e in
                     add_set ep il `contains` be))
-  = admit()
+  = let be = blum_add_elem il i in
+    let ep = be.t.e in
+    let ail = add_il ep il in
+    let asq = i_seq ail in
+    let fm = IF.to_fm (is_blum_add_epoch_ifn #vspec #n ep) (blum_add_elem_src_ifn #vspec #n) in
+    let j = IF.filter_map_map fm il i in
+
+    index_prop ail j;
+    assert(S.index asq j = be);
+    mset_contains_seq_element #_ #(ms_hashfn_dom_cmp vspec.app) asq j
 
 let some_add_elem_idx
   (#vspec #n:_)
@@ -24,13 +98,27 @@ let some_add_elem_idx
   (be: ms_hashfn_dom vspec.app {let ep = be.t.e in
                                 add_set ep il `contains` be})
   : i: seq_index il {is_blum_add il i /\ be = blum_add_elem il i}
-  = admit()
+  = let ep = be.t.e in
+    let fm = IF.to_fm (is_blum_add_epoch_ifn #vspec #n ep) (blum_add_elem_src_ifn #vspec #n) in
+    let ail = add_il ep il in
+    let asq = i_seq ail in
+    let j = index_of_mselem #_ #(ms_hashfn_dom_cmp vspec.app) asq be in
+    let i = IF.filter_map_invmap fm il j in
+    index_prop ail j;
+    i
 
 let evict_set_contains_each_evict_elem (#vspec #n:_) (il: verifiable_log vspec n) (i: seq_index il{is_blum_evict il i})
   : Lemma (ensures (let be = blum_evict_elem il i in
                     let ep = be.t.e in
                     evict_set ep il `contains` be))
-  = admit()
+  = let be = blum_evict_elem il i in
+    let ep = be.t.e in
+    let eil = evict_il ep il in
+    let es = i_seq eil in
+    let fm = IF.to_fm (is_blum_evict_epoch_ifn #vspec #n ep) (blum_evict_elem_src_ifn #vspec #n) in
+    let j = IF.filter_map_map fm il i in
+    index_prop eil j;
+    mset_contains_seq_element #_ #(ms_hashfn_dom_cmp vspec.app) es j
 
 let evict_set_is_a_set (#vspec #n:_) (ep: epoch) (il: verifiable_log vspec n)
   : Lemma (ensures (is_set (evict_set ep il)) )
@@ -42,7 +130,14 @@ let evict_elem_idx
   (be: ms_hashfn_dom vspec.app {let ep = be.t.e in
                                 evict_set ep il `contains` be})
   : i: seq_index il {is_blum_evict il i /\ be = blum_evict_elem il i}
-  = admit()
+  = let ep = be.t.e in
+    let fm = IF.to_fm (is_blum_evict_epoch_ifn #vspec #n ep) (blum_evict_elem_src_ifn #vspec #n) in
+    let eil = evict_il ep il in
+    let es = i_seq eil in
+    let j = index_of_mselem #_ #(ms_hashfn_dom_cmp vspec.app) es be in
+    let i = IF.filter_map_invmap fm il j in
+    index_prop eil j;
+    i
 
 let lemma_evict_before_add (#vspec #n:_) (itsl: its_log vspec n) (i:seq_index itsl{is_blum_add itsl i}):
   Lemma (ensures (let be = blum_add_elem itsl i in
@@ -83,15 +178,36 @@ let lemma_add_set_mem (#vspec #n:_) (il: verifiable_log vspec n) (i1 i2: seq_ind
                     mem be (add_set ep il) >= 2))
   = admit()
 
+let is_blum_add_of_key (#vspec: verifier_spec) (#n:_) (ep: epoch) (gk: key vspec.app)
+  (il: verifiable_log vspec n) (i: seq_index il)
+  = is_blum_add il i &&
+    (let be = blum_add_elem il i in
+     be.t.e = ep && fst be.r = gk)
+
+let is_blum_add_of_key_ifn (#vspec: verifier_spec) (#n:_) (ep: epoch) (gk: key vspec.app)
+  : IF.idxfn_t (gen_seq vspec n) bool
+  = is_blum_add_of_key #vspec #n ep gk
+
+let is_blum_evict_of_key (#vspec: verifier_spec) (#n:_) (ep: epoch) (gk: key vspec.app)
+  (il: verifiable_log vspec n) (i: seq_index il)
+  = is_blum_evict il i &&
+    (let be = blum_evict_elem il i in
+     be.t.e = ep && fst be.r = gk)
+
+let is_blum_evict_of_key_ifn (#vspec: verifier_spec) (#n:_) (ep: epoch) (gk: key vspec.app)
+  : IF.idxfn_t (gen_seq vspec n) bool
+  = is_blum_evict_of_key #vspec #n ep gk
+
 (* add elements of a specific key*)
 let k_add_il (#vspec: verifier_spec) (#n:_) (ep: epoch) (gk: key vspec.app) (il: verifiable_log vspec n)
   : interleaving (ms_hashfn_dom vspec.app) n
-  = admit()
+  = let fm = IF.to_fm (is_blum_add_of_key_ifn #vspec #n ep gk) (blum_add_elem_src_ifn #vspec #n) in
+    IF.filter_map fm il
 
 let k_evict_il (#vspec: verifier_spec) (#n:_) (ep: epoch) (gk: key vspec.app) (il: verifiable_log vspec n)
   : interleaving (ms_hashfn_dom vspec.app) n
-  = admit()
-
+  = let fm = IF.to_fm (is_blum_evict_of_key_ifn #vspec #n ep gk) (blum_evict_elem_src_ifn #vspec #n) in
+    IF.filter_map fm il
 
 let add_set_rel_k_add_set
   (#vspec: verifier_spec)
@@ -101,7 +217,10 @@ let add_set_rel_k_add_set
   (il: verifiable_log vspec n)
   (be: ms_hashfn_dom vspec.app {let gkc,_ = be.r in gkc = gk})
   : Lemma (ensures (mem be (k_add_set ep gk il) = mem be (add_set ep il)))
-  = admit()
+  = let ast = add_set ep il in
+    let astk = k_add_set ep gk il in
+    admit()
+
 
 let evict_set_rel_k_evict_set
   (#vspec: verifier_spec)
